updated it_effect_semA.v

proofs/itrees/it_effect_semA.v
@@ -8,8 +8,13 @@ From ITree Require Import
      Interp.Recursion
      MonadState
      State
-     StateFacts.
+     StateFacts
+     EqAxiom.
 Import Basics.Monads.
+
+Require Import Program.Equality.
+
+From Paco Require Import paco.
 
 From mathcomp Require Import ssreflect ssrfun ssrbool eqtype.
 
@@ -91,6 +96,33 @@ Definition StC_def E (XS: @stateE State -< E) : StC E State :=
     (trigger (@Get State))
     (fun s => trigger (Put State s)).
 
+Definition InstrC_void_def E (XE: ErrEvent -< E) (err: error_data) :
+  InstrC E State FState :=
+  @mk_InstrC asm_op syscall_state sip E State FState (fun _ _ => void1) _
+    (fun x tg ty e => throw err)
+    (fun xs tg o es => throw err)
+    (fun xs o es => throw err)
+    (fun e => throw err)
+    (fun e1 e2 => throw err)
+    (fun x z => throw err)
+    (fun args => throw err)
+    (fun vargs ii => throw err)
+    (fun xs fs s => throw err).
+
+Definition FunC_void_def E (XF: ErrEvent -< E) (err: error_data) :
+  FunC E FState FunDef :=
+  @mk_FunC asm_op syscall_state sip E FState FunDef (fun _ _ => void1) _ 
+    (fun fn fs => throw err)       
+    (fun fd => throw err)       
+    (fun fd fs => throw err)       
+    (fun fd => throw err).       
+
+Definition StC_void_def E (XF: ErrEvent -< E) (err: error_data) :
+  StC E State :=
+  @mk_StC E State (fun _ => void1) _ 
+    (throw err)
+    (fun s => throw err).
+
 End Instances.
 
 
@@ -113,6 +145,7 @@ Definition mk_error_data (s: estate) (e: error) : error_data :=
 Definition mk_error (s: estate) : error_data :=
   mk_error_data s ErrType.
 
+Definition plain_err : error_data := (ErrType, tt).
 
 (*******************************************************)
 
@@ -445,624 +478,220 @@ Definition statefree_interp E T
              +' E) T) : itree _ T :=
   @interp_FunE _ _ p ev _ _ (interp_InstrE p (interp_recc t)).
 *)
+
+Definition isem_interp_up2err (err: error_data) T
+  (t: itree (@InstrE estate fstate
+            +' @FunE fstate fundef
+            +' @stateE estate
+            +' @callE (funname * fstate) fstate
+            +' ErrEvent +' E) T) (s: estate) :
+  itree (ErrEvent +' E) (estate * T) :=
+  @interp_recc asm_op syscall_state sip estate fstate fundef (ErrEvent +' E)
+    (InstrC_void_def inl1 err)
+    (StC_void_def inl1 err)
+    (FunC_void_def inl1 err) _ (@isem_interp_up2rec T t s).
+
+Definition isem2mod {IE FE SE CE EE} :
+  (IE +' FE +' SE +' CE +' EE +' E) ~> 
+           (CE +' IE +' FE +' SE +' EE +' E) :=
+  fun _ e0 => match e0 with
+             | inl1 ie => inr1 (inl1 ie)
+             | inr1 e1 => match e1 with
+               | inl1 fe => inr1 (inr1 (inl1 fe))
+               | inr1 e2 => match e2 with
+                 | inl1 se => inr1 (inr1 (inr1 (inl1 se)))
+                 | inr1 e3 => match e3 with
+                   | inl1 ce => inl1 ce
+                   | inr1 e4 => match e4 with
+                     | inl1 ee => inr1 (inr1 (inr1 (inr1 (inl1 ee))))
+                     | inr1 e5 => inr1 (inr1 (inr1 (inr1 (inr1 e5))))                        end end end end end.     
+
+Definition mod2isem {IE FE SE CE EE} :
+    (CE +' IE +' FE +' SE +' EE +' E) ~> 
+      (IE +' FE +' SE +' CE +' EE +' E) :=
+  fun _ e0 => match e0 with
+             | inl1 ce => inr1 (inr1 (inr1 (inl1 ce)))
+             | inr1 e1 => match e1 with
+               | inl1 ie => inl1 ie
+               | inr1 e2 => match e2 with
+                 | inl1 fe => inr1 (inl1 fe)
+                 | inr1 e3 => match e3 with
+                   | inl1 se => inr1 (inr1 (inl1 se))
+                   | inr1 e4 => match e4 with
+                     | inl1 ee => inr1 (inr1 (inr1 (inr1 (inl1 ee))))
+                     | inr1 e5 => inr1 (inr1 (inr1 (inr1 (inr1 e5))))                        end end end end end.     
+
+Definition isem2mod_tr {IE FE SE CE EE} T
+  (t: itree (IE +' FE +' SE +' CE +' EE +' E) T) :
+  itree (CE +' IE +' FE +' SE +' EE +' E) T :=
+  translate isem2mod t.
+      
+Definition mod2isem_tr {IE FE SE CE EE} T
+  (t: itree (CE +' IE +' FE +' SE +' EE +' E) T) :
+  itree (IE +' FE +' SE +' CE +' EE +' E) T :=
+  translate mod2isem t.
+
+Lemma isem_mod_equiv T
+  (t: itree (@InstrE estate fstate
+            +' @FunE fstate fundef
+            +' @stateE estate
+            +' @callE (funname * fstate) fstate
+            +' ErrEvent +' E) T) (s: estate) :
+  eutt eq (isem_interp_up2err plain_err t s) (interp_up2err (isem2mod_tr t) s).
+Proof.
+(*  unfold isem_interp_up2err, isem_interp_up2rec,
+    interp_up2err, interp_up2state.
+  unfold isem2mod_tr.
+*)
+(* Check @itree_eta_.
+  @itree_eta_
+     : forall (E : Type -> Type) (R : Type) (t : itree E R),
+       t ≅ {| _observe := _observe t |} *)
+(* Check @itree_eta.
+ @itree_eta
+     : forall (E : Type -> Type) (R : Type) (t : itree E R),
+       t ≅ {| _observe := observe t |} *)
+
+  unfold isem_interp_up2err, isem_interp_up2rec,
+    interp_up2err, interp_up2state, Interp_recc, interp_recc.
+
+(* setoid_rewrite interp_mrec_as_interp at 1. *)
+(*  
+  remember (interp_mrec _ _) as X1.
+  remember (interp_mrec _ _) as X2.
+  assert (eutt eq X1 X2) as X1eq. 
+  { inv HeqX1; reflexivity. }
+  rewrite HeqX1.
+  clear HeqX1.
+  inv HeqX2.
+  
+  setoid_rewrite interp_mrec_as_interp in X1eq.
+  unfold isem2mod_tr in X1eq.
+  setoid_rewrite interp_translate in X1eq.
+*)
+  unfold run_state.
+  setoid_rewrite interp_interp.
+  unfold interp_state.
+
+(*  
+  revert X1eq.
+  revert X1.
+*)
+  revert s t.
+
+  ginit; gcofix CIH.
+  intros s t.
+  
+  setoid_rewrite (itree_eta_ t).
+
+  assert (exists ot, eq_itree eq t {| _observe := ot |}) as H.
+  { setoid_rewrite (itree_eta t).
+    exists (observe t).
+    reflexivity.
+  }
+
+  destruct H as [ot H].
+  setoid_rewrite (itree_eta t) in H.
+
+  punfold H; red in H.
+  simpl in *.
+  hinduction H before CIH; try congruence.
+
+  { intros s. 
+    gstep; red.
+    unfold interp_InstrE, interp_FunE; simpl.
+    econstructor; auto.
+  }
+
+  { pclearbot; intros s.
+    gstep; red.
+    unfold interp_InstrE, interp_FunE, run_state; simpl.
+    econstructor.
+    gfinal. left.
+    eapply CIH.
+  }
+  
+  { pclearbot; intros s.
+
+    unfold isem2mod_tr.
+    setoid_rewrite translate_vis.
+    setoid_rewrite unfold_interp_mrec at 2. simpl.
+    setoid_rewrite interp_vis.
+    setoid_rewrite interp_state_bind.
+    setoid_rewrite interp_mrec_bind.
+   
+    destruct e as [ie | e]. simpl.
+    
+    { (* destruct ie eqn: eq_ie. *)
+      setoid_rewrite interp_vis.
+      setoid_rewrite interp_state_bind.
+      setoid_rewrite interp_state_tau.
+      setoid_rewrite interp_tau.
+      setoid_rewrite interp_state_tau.
+
+      set (W1 := interp_mrec _ _).
+      set (W2 := interp_state _ _ _).
+
+      guclo eqit_clo_bind.
+      econstructor.
+      { instantiate (1:= eq).
+        subst W1 W2.
+        unfold ext_handle_InstrE.
+        unfold handle_InstrE; simpl.
+
+        setoid_rewrite interp_mrec_as_interp.
+        unfold interp_state.
+        repeat setoid_rewrite unfold_interp; simpl.
+      
+        destruct ie eqn: ie_eq; simpl.
+        { eapply eqit_Tau_l.
+          clear t.
+          unfold MonadIter_itree; simpl.
+          setoid_rewrite bind_trigger.
+          setoid_rewrite interp_state_vis.
+          setoid_rewrite interp_iter.
+          unfold CategoryOps.iter.
+          unfold Iter_Kleisli.
+          unfold Basics.iter.
+          unfold MonadIter_itree; simpl.
+          setoid_rewrite interp_state_tau.
+          unfold ITree.map; simpl.
+
+          admit.
+        }
+        admit. 
+        admit.
+        admit.
+        admit.
+        admit.
+        admit.
+        admit.
+        admit.
+      }
+
+      { intros u1 u2 H.
+        inv H.
+
+        setoid_rewrite unfold_interp_mrec at 1.
+        simpl.
+        gstep; red.
+        eapply EqTauR; eauto.
+        
+        eapply EqTau.
+        gfinal; left.
+        eapply CIH.
+      }  
+    }  
+
+    admit.
+Admitted. 
   
 End SemDefs.
 
-
-Section SemDefs2.
-
-Context {E : Type -> Type}
-  {XE : ErrEvent -< E}
-  {SX : @stateE estate -< E} 
-  {XI : @InstrE asm_op syscall_state sip estate fstate -< E}
-  {XF : @FunE asm_op syscall_state sip fstate fundef -< E}
-  {XC : @callE (funname * fstate) fstate -< E}.
-
-Context (p : prog) (ev : extra_val_t).
-
-Definition full_interpX E0 T
-  (t: itree E T) (s: estate) :
-  itree E0 (execS (estate * T)) :=
-  full_interp p ev t s.
-  
-End SemDefs2. 
-
-
-
-Definition full_interp E0 T
-  (t: itree (@callE (funname * fstate) fstate
-             +' @InstrE asm_op syscall_state sip estate fstate
-             +' @FunE asm_op syscall_state sip fstate fundef
-             +' @stateE estate
-             +' ErrEvent +' E0) T) (s: estate) :
-  itree E0 (execS (estate * T)) :=
-  interp_Err (run_state (interp_FunE p ev (interp_InstrE p (interp_recc t))) s).
- 
-
- 
-
-
-
-
-
-(****************************************************************)
-
-(* state events (similar to those provided by the library, 
-   could be specialized to estate) *)
-Variant StE : Type -> Type :=
-  | GetSE : StE State
-  | PutSE : State -> StE unit.                      
-
-(* instruction events. InitFState allows storing instr_info in FState
-*)
-Variant InstrE : Type -> Type :=
-  | AssgnE : lval -> assgn_tag -> stype -> pexpr -> InstrE unit
-  | OpnE : lvals -> assgn_tag -> sopn -> pexprs -> InstrE unit
-  | SyscallE : lvals -> syscall_t -> pexprs -> InstrE unit
-  | EvalCond (e: pexpr) : InstrE bool
-  | EvalBound (e: pexpr) : InstrE Z
-  | WriteIndex (x: var_i) (z: Z) : InstrE unit
-  | EvalArgs (args: pexprs) : InstrE pexprs                
-  | InitFState (args: pexprs) : instr_info -> InstrE FState
-  | RetVal (xs: lvals) (fs: FState) (s: State) : InstrE unit.
-
-(* function call events *)
-Variant FunE : Type -> Type :=
-  | GetFunDef (fn: funname) (fs: FState) : FunE FunDef
-  | GetFunCode (fd: FunDef) : FunE cmd          
-  | InitFunCall (fd: FunDef) (fs: FState) : FunE FState                     
-  | FinalizeFunCall (fd: FunDef) : FunE FState.
-
-(* Notation rec_call f fs := (trigger_inl1 (Call (f, fs))). *)
-Local Notation continue_loop := (ret (inl tt)).
-Local Notation exit_loop := (ret (inr tt)).
-
-(* folding instruction semantics on commands (as there's no state,
-   this could actually be simply map) *)
-Definition isem_foldr {E} (sem_i: instr -> itree E unit) (c: cmd) :
-    itree E unit :=
-  foldr (fun i k => sem_i i ;; k) (Ret tt) c.
-
-Definition isem_for_round {E} (sem_i: instr -> itree E unit)
-  (wrt: Z -> itree E unit)                        
-  (i : var_i) (c : cmd) (w: Z) (k: itree E unit) : itree E unit :=
-  wrt w ;; isem_foldr sem_i c ;; k.
-
-Definition isem_for_loop  {E} (sem_i: instr -> itree E unit)
-  (wrt: Z -> itree E unit) 
-  (i : var_i) (c : cmd) (ls : list Z)
-  : itree E unit :=
-  foldr (isem_for_round sem_i wrt i c) (Ret tt) ls.
-
-Definition isem_while_round {E} (sem_i: instr -> itree E unit)
-  (cnd: pexpr -> itree E bool) 
-  (c1 : cmd) (e : pexpr) (c2 : cmd) :
-    itree E (unit + unit) :=
-  isem_foldr sem_i c1 ;;
-  b <- cnd e ;;
-  if b then isem_foldr sem_i c2 ;; continue_loop 
-  else exit_loop.
-
-Definition isem_while_loop {E} (sem_i: instr -> itree E unit)
-  (cnd: pexpr -> itree E bool)
-  (c1 : cmd) (e: pexpr) (c2: cmd) :
-    itree E unit :=
-  ITree.iter (fun _ => isem_while_round sem_i cnd c1 e c2) tt.
-
-Notation recCall := (callE (funname * FState) FState).
-
-Section SemRec.
-
-Context {E} {XI : InstrE -< E} {XS: StE -< E}.
-
-(* semantics of instructions *)
-Fixpoint isem_instr (i : instr) : itree (recCall +' E) unit :=
-  let: (MkI ii ir) := i in
-  match ir with
-  | Cassgn x tg ty e => trigger (AssgnE x tg ty e)
-
-  | Copn xs tg o es => trigger (OpnE xs tg o es)
-
-  | Csyscall xs o es => trigger (SyscallE xs o es) 
-                                
-  | Cif e c1 c2 =>
-    b <- trigger (EvalCond e) ;;
-    isem_foldr isem_instr (if b then c1 else c2) 
-               
-  | Cwhile a c1 e ii0 c2 =>
-      isem_while_loop isem_instr (fun e => trigger (EvalCond e))
-        c1 e c2 
-
-  | Cfor i (d, lo, hi) c =>
-    lo_b <- trigger (EvalBound lo) ;;
-    hi_b <- trigger (EvalBound hi) ;;   
-    isem_for_loop isem_instr (fun w => trigger (WriteIndex i (Vint w)))
-      i c (wrange d lo_b hi_b) 
-
-  | Ccall xs fn args =>
-    s0 <- trigger GetSE ;;  
-    vargs <- trigger (EvalArgs args) ;;
-    fs0 <- trigger (InitFState vargs ii) ;;
-    fs1 <- trigger_inl1 (Call (fn, fs0)) ;; 
-    (* discard current state, use s0 instead *)
-    trigger (RetVal xs fs1 s0)
-  end.
-
-(* semantics of commands *)
-Definition isem_cmd c := isem_foldr isem_instr c.
-
-Lemma fold_cmd c: isem_cmd c = isem_foldr isem_instr c.
-Proof. by reflexivity. Qed. 
-
-Section SemFun.
-
-Context {XF: FunE -< E}.  
-
-(* semantics of function calls *)
-Definition isem_fcall (fn : funname) (fs : FState) :
-  itree (recCall +' E) FState :=
-  fd <- trigger (GetFunDef fn fs) ;;  
-  c <- trigger (GetFunCode fd) ;;
-  trigger (InitFunCall fd fs) ;;
-  isem_cmd c ;;
-  trigger (FinalizeFunCall fd).
-
-(************************************************************)
-(* full function semantics *)
-
-(* handler of recCall events *)
-Definition handle_recc : recCall ~> itree (recCall +' E) :=
- fun T (rc : recCall T) =>
-   match rc with
-   | Call (fn, fs) => isem_fcall fn fs
-   end.
-
-(* intepreter of recCall events *)
-Definition interp_recc T (t: itree (recCall +' E) T) : itree E T :=
-  interp_mrec handle_recc t.
-
-(* recCall interpreter of instructions *)
-Definition denote_instr (i: instr) : itree E unit :=
-  interp_recc (isem_instr i).
-
-(* recCall interpreter of commands *)
-Definition denote_cmd (c: cmd) : itree E unit :=
-  interp_recc (isem_cmd c).
-
-(* recCall interpreter of function calls (corresponds to: isem_fun) *)
-Definition denote_fun (fn : funname) (fs : FState) : itree E FState :=
-  interp_recc (isem_fcall fn fs).
-
-(* function semantics, expressed with rec rather than interp_mrec *)
-Definition denote_fun' (fn : funname) (fs : FState) : itree E FState :=
-  rec (uncurry isem_fcall) (fn, fs). 
-
-(* corresponds to: isem_fun_body with the sem_fun_full instance *) 
-Definition denote_fcall (fn : funname) (fs : FState) :
-  itree E FState :=
-  fd <- trigger (GetFunDef fn fs) ;;  
-  c <- trigger (GetFunCode fd) ;;
-  trigger (InitFunCall fd fs) ;;
-  denote_cmd c ;;
-  trigger (FinalizeFunCall fd).
-
-
-(********************************************************************)
-(* blank function semantics *)
-
-Definition rec_call (f : funname) (fs : FState) :
-   itree (recCall +' E) FState := trigger_inl1 (Call (f, fs)).
-
-(* fully blank semantics (does nothing) *)
-Definition denote_fun_blank' (fn : funname) (fs : FState) : itree E FState :=
-  rec (uncurry rec_call) (fn, fs). 
-
-(* blank handler of recCall events *)
-Definition handle_recc_blank : recCall ~> itree (recCall +' E) :=
- fun T (rc : recCall T) =>
-   match rc with
-   | Call (fn, fs) => trigger_inl1 (Call (fn, fs))
-   end.
-
-(* uninterpreted function semantics *)
-Definition denote_fun_blank (fn : funname) (fs : FState) : itree E FState :=
-  interp_mrec handle_recc_blank (isem_fcall fn fs).
-
-(**********************************************************************)
-
-Lemma denote_fun_eutt (fn : funname) (fs : FState) :
-  eutt eq (denote_fun' fn fs) (denote_fun fn fs).
-Proof. by reflexivity. Qed.  
-
-Lemma isem_cmd_cons i c :
-  eutt eq (isem_cmd (i :: c))
-          (isem_instr i ;; isem_cmd c).       
-Proof. by reflexivity. Qed.
-
-Lemma isem_cmd_cat c1 c2 :
-  eutt eq (isem_cmd (c1 ++ c2))
-          (isem_cmd c1 ;; isem_cmd c2).       
-Proof.
-  induction c1; simpl.
-  - rewrite bind_ret_l; reflexivity.     
-  - setoid_rewrite bind_bind.
-    setoid_rewrite IHc1; reflexivity.
-Qed.
-
-Lemma denote_cmd_cons i c :
-  eutt eq (denote_cmd (i :: c))
-          (denote_instr i ;; denote_cmd c).       
-Proof.
-  setoid_rewrite interp_mrec_as_interp; simpl.
-  setoid_rewrite interp_bind; reflexivity.
-Qed.
-
-Lemma denote_cmd_cat c1 c2 :
-  eutt eq (denote_cmd (c1 ++ c2))
-          (denote_cmd c1 ;; denote_cmd c2).       
-Proof.
-  unfold denote_cmd, interp_recc; simpl.
-  setoid_rewrite interp_mrec_as_interp; simpl.
-  setoid_rewrite isem_cmd_cat; simpl.
-  setoid_rewrite interp_bind; reflexivity.
-Qed.
-  
-Lemma denote_cmd_cat' c1 c2 :
-  eutt eq (denote_cmd (c1 ++ c2))
-          (denote_cmd c1 ;; denote_cmd c2).       
-Proof.
-  induction c1; simpl.
-  - unfold denote_cmd at 2; simpl.
-    setoid_rewrite interp_mrec_as_interp; simpl.
-    setoid_rewrite interp_ret.
-    setoid_rewrite bind_ret_l; reflexivity.
-  - setoid_rewrite <- app_comm_cons; simpl.
-    setoid_rewrite interp_mrec_as_interp; simpl.
-    setoid_rewrite interp_bind.
-    setoid_rewrite bind_bind.
-    eapply eqit_bind; try reflexivity.
-    unfold pointwise_relation; intros _.
-    setoid_rewrite <- interp_mrec_as_interp; auto.
-Qed.
-  
-Lemma isem_cmd_while ii al c e inf c':
-  isem_cmd [:: MkI ii (Cwhile al c e inf c')] 
-  ≈
-  isem_cmd (c ++ [:: MkI ii (Cif e (c' ++ [:: MkI ii (Cwhile al c e inf c')])
-                               [::])]).
-Proof.
-  rewrite isem_cmd_cat. 
-  unfold isem_cmd at 1; simpl.
-  unfold isem_while_loop; simpl.
-  setoid_rewrite bind_ret_r_unit.
-  setoid_rewrite unfold_iter; simpl.
-  unfold isem_while_round; simpl.
-  setoid_rewrite bind_bind.
-  setoid_rewrite bind_bind.
-  eapply eqit_bind; try reflexivity.
-  unfold pointwise_relation; simpl.
-  intro u; destruct u.
-  eapply eqit_bind; try reflexivity.
-  unfold pointwise_relation; simpl.
-  intro b; destruct b; simpl.
-  - setoid_rewrite bind_bind.
-    setoid_rewrite <- fold_cmd at 2.
-    rewrite isem_cmd_cat.
-    eapply eqit_bind; try reflexivity.
-    unfold pointwise_relation; simpl.
-    intro u; destruct u; simpl.
-    setoid_rewrite bind_ret_l.
-    eapply eqit_Tau_l.
-    setoid_rewrite bind_ret_r_unit; reflexivity.  
-  - setoid_rewrite bind_ret_l; reflexivity.
-Qed.    
-  
-Lemma denote_cmd_while ii al c e inf c':
-  denote_cmd [:: MkI ii (Cwhile al c e inf c')] 
-  ≈
-  denote_cmd (c ++ [:: MkI ii (Cif e (c' ++ [:: MkI ii (Cwhile al c e inf c')])
-                               [::])]).
-Proof.
-  unfold denote_cmd, interp_recc.
-  setoid_rewrite interp_mrec_as_interp.
-  setoid_rewrite isem_cmd_while; reflexivity.
-Qed.  
-
-Lemma interp_isem_cmd c :
-  eutt (E:=E) eq (interp_recc (isem_cmd c)) (isem_foldr denote_instr c).
-Proof.
-  apply:
-   (cmd_rect
-    (Pr := fun ir => forall ii,
-       eutt (E:=E) eq (interp_recc (isem_instr (MkI ii ir)))
-                      (denote_instr (MkI ii ir)))
-    (Pi := fun i => 
-       eutt (E:=E) eq (interp_recc (isem_instr i))
-                      (denote_instr i))
-    (Pc := fun c => 
-       eutt (E:=E) eq (interp_recc (isem_cmd c))
-                      (isem_foldr denote_instr c)));
-    clear c; simpl; try (intros; reflexivity).
-  - setoid_rewrite interp_mrec_as_interp.
-    setoid_rewrite interp_ret; reflexivity.
-  - intros i c H H0.
-    setoid_rewrite interp_mrec_as_interp; simpl.
-    setoid_rewrite interp_bind.
-    eapply eqit_bind.
-    setoid_rewrite <- interp_mrec_as_interp; reflexivity.
-    unfold pointwise_relation; intro u; destruct u.
-    rewrite <- H0.
-    setoid_rewrite <- interp_mrec_as_interp; reflexivity.
-Qed.    
-
-Lemma isem_call_unfold (fn : funname) (fs : FState) :
-  denote_fun fn fs ≈ denote_fcall fn fs.
-Proof.
-  unfold denote_fun, interp_recc, denote_fcall.
-  setoid_rewrite interp_mrec_as_interp.
-  unfold isem_fcall.
-  rewrite interp_bind.
-  eapply eqit_bind.
-  - setoid_rewrite interp_trigger; simpl; reflexivity.
-  - unfold pointwise_relation; intro fd.
-    rewrite interp_bind.
-    eapply eqit_bind.
-  - setoid_rewrite interp_trigger; simpl; reflexivity.  
-  - unfold pointwise_relation; intro c.
-    rewrite interp_bind.
-    eapply eqit_bind.
-  - setoid_rewrite interp_trigger; simpl; reflexivity.    
-  - unfold pointwise_relation; intro fs1.
-    rewrite interp_bind.
-    eapply eqit_bind; try reflexivity.
-  - unfold pointwise_relation; intro u.
-    setoid_rewrite interp_trigger; simpl; reflexivity.    
-Qed.    
-    
-Section Inline.
-
-(* inline info is included in FState *)  
-Context {do_inline :
-    FState -> funname (* caller *) -> funname (* callee *) -> bool}.
-
-(* conditional inliner action *)
-Definition inliner
- (ctx : forall T : Type, recCall T -> itree (recCall +' E) T)
- (caller: funname) (callee: funname) (fs: FState) :
-  itree (recCall +' E) FState :=
-  if do_inline fs caller callee then ctx FState (Call (callee, fs))
-(* Interpret the top call but not the inner ones *)
-     else trigger_inl1 (E:=E) (Call (callee, fs)).
-(* Do not interpret the call, simply retrigger the event *)
-
-(* given the caller Name and the callee Event, lifts inliner to a
-   handler with polymorphic return type *)
-Definition inline_handleNE
-  (ctx : forall T : Type, recCall T -> itree (recCall +' E) T)
-  (caller: funname) T (cle: recCall T) : itree (recCall +' E) T :=
-  match cle with
-  | Call (fn, fs) => inliner ctx caller fn fs end. 
-
-(* similar, given caller Event and callee Event *)
-Definition inline_handleEE
-  (ctx : forall T : Type, recCall T -> itree (recCall +' E) T)
-  T1 (clr: recCall T1) T2 (cle: recCall T2) : itree (recCall +' E) T2 :=
-  match clr with
-  | Call (caller, _) => inline_handleNE ctx caller cle end. 
-
-(* folds the inliner on an itree *)
-Definition inline_handleE 
-        (ctx : forall T : Type, recCall T -> itree (recCall +' E) T)
-        (T1 : Type) (d1 : recCall T1) :
-  itree (recCall +' E) ~> itree (recCall +' E) := 
-  interp (ext_r_handler (inline_handleEE ctx d1)).
-
-(* the proper inline handler: given a caller, it inteprets its body
-   with the inliner *) 
-Definition inline_handle 
-        (ctx : forall T : Type, recCall T -> itree (recCall +' E) T)
-        (T1 : Type) (d1 : recCall T1) : itree (recCall +' E) T1 := 
-  (inline_handleE ctx d1) T1 (ctx T1 d1).
-
-(* makes the definition concrete *)
-Definition inline_handle_recc : forall (T1 : Type) (d1 : recCall T1),
-  itree (recCall +' E) T1 := inline_handle handle_recc.
-
-Lemma isem_call_inline T (e: recCall T) :
-  mrec handle_recc e ≈ mrec inline_handle_recc e.
-Proof.
-  unfold handle_recc, inline_handle_recc.  
-  set cond := fun  T1 (d1: recCall T1) T2 (d2: recCall T2) =>
-    match d1, d2 with
-    | Call (caller, _), Call (callee, fs) => do_inline fs caller callee
-    end.
-  rewrite (mrec_loop2 cond).
-  set F := (X in ctx2_cond _ X).  
-  set G := (inline_handle _).
-  assert (forall T0 (e0: recCall T0),
-             eutt eq (ctx2_cond cond F e0) (G _ e0)) as H1.
-  { intros T0 [[fn0 fs0]]; subst F G cond.
-    unfold ctx2_cond, Handler.cat, ctx_cond, Handler.case_,
-      inline_handle, inline_handleE, ext_r_handler,
-      inline_handleEE, inline_handleNE, handle_recc, inliner; simpl.
-    eapply eutt_interp; try reflexivity.
-    unfold eq2, Eq2_Handler, eutt_Handler, Relation.i_pointwise.
-    intros T1 [[[fn1 fs1]] | e1]; simpl; try reflexivity.
-  }
-  unfold mrec; eapply Proper_interp_mrec; eauto.
-Qed.
-    
-End Inline.  
-
-End SemFun.
-
-End SemRec.
-
-
-(**********************************************************************)
-
-Class sem_Fun (E : Type -> Type) :=
-  { sem_fun : funname -> FState -> itree E FState }.
-
-#[global]
-Instance sem_fun_rec (E : Type -> Type) : sem_Fun (recCall +' E) | 0 :=
-  {| sem_fun := @rec_call E |}.
-  
-Section SemPRec.
-
-Context {E} {XI : InstrE -< E} {XS: StE -< E} {sem_F : sem_Fun E }.
-  
-Context (sem_i: instr -> itree E unit).
-
-(* semantics of instructions, abstracting on function calls (through
-   sem_fun) *)
-Fixpoint isem_i_body (i : instr) : itree E unit :=
-  let: (MkI ii i) := i in
-  match i with
-  | Cassgn x tg ty e => trigger (AssgnE x tg ty e)
-
-  | Copn xs tg o es => trigger (OpnE xs tg o es)
-
-  | Csyscall xs o es => trigger (SyscallE xs o es) 
-                                
-  | Cif e c1 c2 =>
-    b <- trigger (EvalCond e) ;;
-    isem_foldr isem_i_body (if b then c1 else c2) 
-               
-  | Cwhile a c1 e i c2 =>
-      isem_while_loop isem_i_body (fun e => trigger (EvalCond e))
-        c1 e c2 
-
-  | Cfor i (d, lo, hi) c =>
-    lo_b <- trigger (EvalBound lo) ;;
-    hi_b <- trigger (EvalBound hi) ;;   
-    isem_for_loop isem_i_body (fun w => trigger (WriteIndex i (Vint w)))
-      i c (wrange d lo_b hi_b) 
-
-  | Ccall xs fn args =>
-    s0 <- trigger GetSE ;;  
-    vargs <- trigger (EvalArgs args) ;;
-    fs0 <- trigger (InitFState vargs ii) ;;
-    fs1 <- sem_fun fn fs0 ;; 
-    (* discard current state, use s0 instead *)
-    trigger (RetVal xs fs1 s0)
-(* | _ => throw err end. *)
-  end.
-
-(* similar, for commands *)
-Definition isem_c_body c := isem_foldr isem_i_body c.
-
-Section SemPFun.
-
-Context {XF: FunE -< E}.  
-
-Definition isem_fun_body (fn : funname) (fs : FState) : itree E FState :=
-  fd <- trigger (GetFunDef fn fs) ;;  
-  c <- trigger (GetFunCode fd) ;;
-  trigger (InitFunCall fd fs) ;;
-  isem_c_body c ;; 
-  trigger (FinalizeFunCall fd).
-
-End SemPFun.
-
-End SemPRec.
-
-Section SemA.
-  
-Context {E}
-  {XE : ErrEvent -< E} {XI : InstrE -< E} {XS: StE -< E}.
-
-Context {XF: FunE -< E}.
-
-Context (sem_i: instr -> itree (recCall +' E) unit).
-
-(************************************************************)
-(* uninterpreted function semantics *)
-
-(* semantics of instructions parametrized by recCall events *)
-Definition isem_i_rec (i : instr) : itree (recCall +' E) unit :=
-  isem_i_body i.
-  
-Definition isem_cmd_rec (c : cmd) : itree (recCall +' E) unit :=
-  isem_c_body c.
-
-Definition isem_fun_rec 
-  (fn : funname) (fs : FState) : itree (recCall +' E) FState :=
-  isem_fun_body fn fs.
-
-(************************************************************)
-(* full function semantics *)
-
-(* handler of recCall events *)
-Definition handle_recCall :
-   recCall ~> itree (recCall +' E) :=
- fun T (rc : recCall T) =>
-   match rc with
-   | Call (fn, fs) => isem_fun_rec fn fs
-   end.
-
-(* intepreter of recCall events *)
-Definition interp_recCall T (t: itree (recCall +' E) T) : itree E T :=
-  interp_mrec handle_recCall t.
-
-(* intepreter of recCall events for functions, giving us the recursive
-   semantics of functions *)
-Definition isem_fun (fn : funname) (fs : FState) : itree E FState :=
-  mrec handle_recCall (Call (fn, fs)).
-
-#[global]
-Instance sem_fun_full : sem_Fun E | 100 :=
-  {| sem_fun := isem_fun |}.
-
-(* recursive semantics of instructions *)
-Definition isem_i (i : instr) : itree E unit :=
-  isem_i_body i.
-
-(* similar, for commands *)
-Definition isem_c (c : cmd) : itree E unit :=
-  isem_c_body c.
-
-(************************************************************)
-(* blank function semantics *)
-
-(* blank recCall handler *)
-Definition handle_recCallB :
-   recCall ~> itree (recCall +' E) :=
- fun T (rc : recCall T) =>
-   match rc with
-   | Call (fn, fs) => rec_call fn fs
-   end.
-
-(* blank recCall interpreter (non-terminating) *)
-Definition interp_recCallB T (t: itree (recCall +' E) T) : itree E T :=
-  interp_mrec handle_recCallB t.
-
-(* blank function semantics *)
-Definition isem_funB (fn : funname) (fs : FState) : itree E FState :=
-  mrec handle_recCallB (Call (fn, fs)).
-
-(*********************************************************************)
-
-Lemma isem_fun_rec_eutt (fn : funname) (fs : FState) :
-  eutt eq (isem_fun_rec fn fs) (isem_fcall fn fs).
-Proof. by reflexivity. Qed.
-
-Lemma interp_recCall_eutt T (t: itree (recCall +' E) T) :
-  eutt eq (interp_recCall t) (interp_recc t).
-Proof.
-  unfold interp_recCall, interp_recc.
-  eapply interp_mrec_eqit with (VRel := @eq); try reflexivity.
-  intros V k1 k2 H v1 v2 H0.
-  inv H0; eauto.
-Qed.
-
-End SemA.
-  
-End Sem1.
-
 End Asm2.
-
+  
 End Asm1.
+
 
 
 
